reintroduce inclusive for liveness trimmed analysis; nolonger think non-uniqueness is a problem since congruence is with repsect to a particular dynamic channel

theory/Static_Communication_Analysis_B.thy
@@ -5,7 +5,7 @@ theory Static_Communication_Analysis_B
     Static_Communication_Analysis 
 begin
 
-datatype edge_label = ENext | ESpawn | ECall | EReturn var
+datatype edge_label = ENext | ESpawn | ESend var | ECall | EReturn var
 
 type_synonym flow_label = "(node_label \<times> edge_label \<times> node_label)"
 
@@ -439,9 +439,65 @@ inductive may_be_static_live_path :: "abstract_value_env \<Rightarrow> flow_set 
     may_be_static_live_path V F Ln Lx start isEnd path
   "
 
+
+
+inductive may_be_inclusive :: "abstract_path \<Rightarrow> abstract_path \<Rightarrow> bool" (infix "\<asymp>" 55) where
+  Prefix1: "
+    prefix \<pi>\<^sub>1 \<pi>\<^sub>2 \<Longrightarrow>
+    \<pi>\<^sub>1 \<asymp> \<pi>\<^sub>2
+  " |
+  Prefix2: "
+    prefix \<pi>\<^sub>2 \<pi>\<^sub>1 \<Longrightarrow>
+    \<pi>\<^sub>1 \<asymp> \<pi>\<^sub>2
+  " |
+  Spawn1: "
+    \<pi> @ (NLet x, ESpawn) # \<pi>\<^sub>1 \<asymp> \<pi> @ (NLet x, ENext) # \<pi>\<^sub>2
+  " |
+  Spawn2: "
+    \<pi> @ (NLet x, ENext) # \<pi>\<^sub>1 \<asymp> \<pi> @ (NLet x, ESpawn) # \<pi>\<^sub>2
+  " |
+  Send1: "
+    \<pi> @ (NLet x, ESend xE) # \<pi>\<^sub>1 \<asymp> \<pi> @ (NLet x, ENext) # \<pi>\<^sub>2
+  " |
+  Send2: "
+    \<pi> @ (NLet x, ENext) # \<pi>\<^sub>1 \<asymp> \<pi> @ (NLet x, ESend xE) # \<pi>\<^sub>2
+  "
+
+lemma may_be_inclusive_commut: "
+  path\<^sub>1 \<asymp> path\<^sub>2 \<Longrightarrow> path\<^sub>2 \<asymp> path\<^sub>1
+"
+ apply (erule may_be_inclusive.cases; auto)
+  apply (simp add: Prefix2)
+  apply (simp add: Prefix1)
+  apply (simp add: Spawn2)
+  apply (simp add: Spawn1)
+  apply (simp add: Send2)
+  apply (simp add: Send1)
+done
+
+
+lemma may_be_inclusive_preserved_under_unordered_extension: "
+  \<not> prefix path\<^sub>1 path\<^sub>2 \<Longrightarrow> \<not> prefix path\<^sub>2 path\<^sub>1 \<Longrightarrow> path\<^sub>1 \<asymp> path\<^sub>2 \<Longrightarrow> path\<^sub>1 @ [l] \<asymp> path\<^sub>2
+"
+ apply (erule may_be_inclusive.cases; auto)
+  apply (simp add: Spawn1)
+  apply (simp add: Spawn2)
+  apply (simp add: Send1)
+  apply (simp add: Send2)
+done
+
+lemma may_be_inclusive_preserved_under_unordered_double_extension: "
+  path\<^sub>1 \<asymp> path\<^sub>2 \<Longrightarrow> \<not> prefix path\<^sub>1 path\<^sub>2 \<Longrightarrow> \<not> prefix path\<^sub>2 path\<^sub>1 \<Longrightarrow> path\<^sub>1 @ [l1] \<asymp> path\<^sub>2 @ [l2]
+"
+by (metis may_be_inclusive_commut may_be_inclusive_preserved_under_unordered_extension prefix_append prefix_def)
+
 inductive singular :: "abstract_path \<Rightarrow> abstract_path \<Rightarrow> bool" where
   equal: "
     \<pi>\<^sub>1 = \<pi>\<^sub>2 \<Longrightarrow> 
+    singular \<pi>\<^sub>1 \<pi>\<^sub>2
+  " |
+  exclusive: "
+    \<not> (\<pi>\<^sub>1 \<asymp> \<pi>\<^sub>2) \<Longrightarrow> 
     singular \<pi>\<^sub>1 \<pi>\<^sub>2
   "
 
@@ -449,8 +505,11 @@ inductive noncompetitive :: "abstract_path \<Rightarrow> abstract_path \<Rightar
   ordered: "
     ordered \<pi>\<^sub>1 \<pi>\<^sub>2 \<Longrightarrow> 
     noncompetitive \<pi>\<^sub>1 \<pi>\<^sub>2
+  " |
+  exclusive: "
+    \<not> (\<pi>\<^sub>1 \<asymp> \<pi>\<^sub>2) \<Longrightarrow> 
+    noncompetitive \<pi>\<^sub>1 \<pi>\<^sub>2
   "
-
 
 
 inductive static_one_shot :: "abstract_value_env \<Rightarrow> exp \<Rightarrow> var \<Rightarrow> bool" where
@@ -642,849 +701,7 @@ lemma no_empty_paths_congruent_mod_chan: "
 done
 
 
-lemma send_path_equality_sound: "
-  path1 = path2 \<Longrightarrow>
-  paths_congruent_mod_chan (\<E>', H') (Ch \<pi> xC) \<pi>1 path1 \<Longrightarrow>
-  paths_congruent_mod_chan (\<E>', H') (Ch \<pi> xC) \<pi>2 path2 \<Longrightarrow>
-  ([[] \<mapsto> \<langle>e;Map.empty;[]\<rangle>], {}) \<rightarrow>* (\<E>', H') \<Longrightarrow> 
-  is_send_path \<E>' (Ch \<pi> xC) \<pi>1 \<Longrightarrow> 
-  is_send_path \<E>' (Ch \<pi> xC) \<pi>2 \<Longrightarrow> 
-  \<pi>1 = \<pi>2
-"
-sorry
-(*
-lemma send_abstract_paths_equal_unordered_implies_dynamic_paths_equal: "
-pathSync = pathSynca \<or> (\<not> pathSynca \<asymp> pathSync) \<Longrightarrow> 
-
-([[] \<mapsto> \<langle>e;Map.empty;[]\<rangle>], {}) \<rightarrow>* (\<E>', H') \<Longrightarrow>
-is_send_path \<E>' (Ch \<pi> xC) \<pi>\<^sub>1 \<Longrightarrow>
-is_send_path \<E>' (Ch \<pi> xC) \<pi>\<^sub>2 \<Longrightarrow>
-
-paths_congruent_mod_chan (\<E>', H') (Ch \<pi> xC) \<pi>\<^sub>1 pathSync \<Longrightarrow>
-paths_congruent_mod_chan (\<E>', H') (Ch \<pi> xC) \<pi>\<^sub>2 pathSynca \<Longrightarrow>
-
-\<pi>\<^sub>1 = \<pi>\<^sub>2
-"
-by (simp add: send_path_equality_sound send_abstract_paths_of_same_run_unordered)
-*)
-(* END *)
-
-
-(* PATH SOUND *)
-
-lemma isnt_path_sound: "
-  \<E>' \<pi> = Some (\<langle>LET x = b in e\<^sub>n;\<rho>;\<kappa>\<rangle>) \<Longrightarrow>
-  \<rho> z \<noteq> None \<Longrightarrow>
-  dynamic_built_on_chan_var \<rho> (Ch \<pi>C xC) z \<Longrightarrow>
-  ([[] \<mapsto> \<langle>e;Map.empty;[]\<rangle>], {}) \<rightarrow>* (\<E>', H') \<Longrightarrow> 
-  (V, C) \<Turnstile>\<^sub>e e \<Longrightarrow>
-  static_chan_liveness V Ln Lx xC e \<Longrightarrow>
-  static_flow_set V F (may_be_static_recv_node_label V e) e \<Longrightarrow>
-  isEnd (NLet x) \<Longrightarrow>
-  \<exists> path . 
-    paths_congruent_mod_chan (\<E>', H') (Ch \<pi>C xC) \<pi> path \<and>
-    may_be_static_live_path V F Ln Lx (NLet xC) isEnd path
-"
-sorry
-
-
-lemma isnt_send_path_sound: "
-  is_send_path \<E>' (Ch \<pi>C xC) \<pi>Sync \<Longrightarrow>
-  ([[] \<mapsto> \<langle>e;Map.empty;[]\<rangle>], {}) \<rightarrow>* (\<E>', H') \<Longrightarrow> 
-  (V, C) \<Turnstile>\<^sub>e e \<Longrightarrow>
-  static_chan_liveness V Ln Lx xC e \<Longrightarrow>
-  static_flow_set V F (may_be_static_recv_node_label V e) e \<Longrightarrow>
-  \<exists> pathSync .
-    (paths_congruent_mod_chan (\<E>', H') (Ch \<pi>C xC) \<pi>Sync pathSync) \<and> 
-    may_be_static_live_path V F Ln Lx (NLet xC) (may_be_static_send_node_label V e xC) pathSync
-"
- apply (unfold is_send_path.simps; auto)
- apply (frule_tac x\<^sub>s\<^sub>c = x\<^sub>s\<^sub>c and \<pi>C = \<pi>C and \<rho>\<^sub>e = \<rho>\<^sub>e in isnt_send_site_sound; auto?)
- apply (frule isnt_path_sound; auto?)
-  apply (auto simp: 
-    dynamic_built_on_chan_var.simps 
-    dynamic_built_on_chan_var_dynamic_built_on_chan_prim_dynamic_built_on_chan_bindee_dynamic_built_on_chan_exp.Send_Evt 
-  )
-done
-
-
-theorem one_shot_sound': "
-  every_two (may_be_static_live_path V F Ln Lx (NLet xC) (may_be_static_send_node_label V e xC)) singular \<Longrightarrow>
-  static_chan_liveness V Ln Lx xC e \<Longrightarrow>
-  static_flow_set V F (may_be_static_recv_node_label V e) e \<Longrightarrow>
-  (V, C) \<Turnstile>\<^sub>e e \<Longrightarrow>
-  ([[] \<mapsto> \<langle>e;Map.empty;[]\<rangle>], {}) \<rightarrow>* (\<E>', H') \<Longrightarrow> 
-  every_two_dynamic_paths (is_send_path \<E>' (Ch \<pi> xC)) op =
-"
-apply (simp add: every_two_dynamic_paths.simps every_two.simps singular.simps; auto)
-apply (metis isnt_send_path_sound send_path_equality_sound)
-done
-
-
-
-theorem one_shot_sound: "
-  \<lbrakk>
-    static_one_shot V e xC;
-    (V, C) \<Turnstile>\<^sub>e e;
-    ([[] \<mapsto> \<langle>e;Map.empty;[]\<rangle>], {}) \<rightarrow>* (\<E>', H')
-  \<rbrakk> \<Longrightarrow>
-  one_shot \<E>' (Ch \<pi> xC)
-"
- apply (erule static_one_shot.cases; auto)
- apply (unfold one_shot.simps)
- apply (simp add: one_shot_sound')
-done
-
-theorem noncompetitive_send_to_ordered_send: "
-  every_two (may_be_static_live_path V F Ln Lx (NLet xC) (may_be_static_send_node_label V e xC)) noncompetitive \<Longrightarrow>
-  static_chan_liveness V Ln Lx xC e \<Longrightarrow>
-  static_flow_set V F (may_be_static_recv_node_label V e) e \<Longrightarrow>
-  (V, C) \<Turnstile>\<^sub>e e \<Longrightarrow>
-  ([[] \<mapsto> \<langle>e;Map.empty;[]\<rangle>], {}) \<rightarrow>* (\<E>', H') \<Longrightarrow>
-  every_two_dynamic_paths (is_send_path \<E>' (Ch \<pi> xC)) ordered
-"
-
-apply (simp add: every_two_dynamic_paths.simps noncompetitive.simps; auto)
-sorry
-
-theorem fan_out_sound: "
-  \<lbrakk>
-    static_fan_out V e xC;
-    (V, C) \<Turnstile>\<^sub>e e;
-    ([[] \<mapsto> \<langle>e;Map.empty;[]\<rangle>], {}) \<rightarrow>* (\<E>', H')
-  \<rbrakk> \<Longrightarrow>
-  fan_out \<E>' (Ch \<pi> xC)
-"
- apply (erule static_fan_out.cases; auto)
- apply (unfold fan_out.simps)
- apply (metis noncompetitive_send_to_ordered_send)
-done
-
-lemma noncompetitive_recv_to_ordered_recv: "
-   every_two (may_be_static_live_path V F Ln Lx (NLet xC) (may_be_static_recv_node_label V e xC)) noncompetitive \<Longrightarrow>
-   static_flow_set V F (may_be_static_recv_node_label V e) e \<Longrightarrow>
-   (V, C) \<Turnstile>\<^sub>e e \<Longrightarrow>
-   ([[] \<mapsto> \<langle>e;Map.empty;[]\<rangle>], {}) \<rightarrow>* (\<E>', H') \<Longrightarrow>
-   every_two_dynamic_paths (is_recv_path \<E>' (Ch \<pi> xC)) ordered
-"
-sorry
-
-
-theorem fan_in_sound: "
-  \<lbrakk>
-    static_fan_in V e xC;
-    (V, C) \<Turnstile>\<^sub>e e;
-    ([[] \<mapsto> \<langle>e;Map.empty;[]\<rangle>], {}) \<rightarrow>* (\<E>', H')
-  \<rbrakk> \<Longrightarrow>
-  fan_in \<E>' (Ch \<pi> xC)
-"
- apply (erule static_fan_in.cases; auto)
- apply (unfold fan_in.simps)
- apply (metis noncompetitive_recv_to_ordered_recv)
-done
-
-
-theorem one_to_one_sound: "
-  \<lbrakk>
-    static_one_to_one V e xC;
-    (V, C) \<Turnstile>\<^sub>e e;
-    ([[] \<mapsto> \<langle>e;Map.empty;[]\<rangle>], {}) \<rightarrow>* (\<E>', H')
-  \<rbrakk> \<Longrightarrow>
-  one_to_one \<E>' (Ch \<pi> xC)
-"
- apply (erule static_one_to_one.cases; auto)
- apply (unfold one_to_one.simps)
- apply (simp add: noncompetitive_recv_to_ordered_recv noncompetitive_send_to_ordered_send)
-done
-(*
-
-
-
-
-inductive static_flow_set :: "abstract_value_env \<Rightarrow> flow_set \<Rightarrow> (var \<Rightarrow> node_label \<Rightarrow> bool) \<Rightarrow> exp \<Rightarrow> bool"  where
-  Result: "
-    static_flow_set V F may_be_recv_site (RESULT x)
-  " |
-  Let_Unit: "
-    \<lbrakk>
-      {(NLet x , ENext, nodeLabel e)} \<subseteq> F;
-      static_flow_set V F may_be_recv_site e
-    \<rbrakk> \<Longrightarrow>
-    static_flow_set V F may_be_recv_site (LET x = \<lparr>\<rparr> in e)
-  " |
-  Let_Chan: "
-    \<lbrakk>
-      {(NLet x, ENext, nodeLabel e)} \<subseteq> F;
-      static_flow_set V F may_be_recv_site e
-    \<rbrakk> \<Longrightarrow>
-    static_flow_set V F may_be_recv_site (LET x = CHAN \<lparr>\<rparr> in e)
-  " |
-  Let_Send_Evt: "
-    \<lbrakk>
-      {(NLet x, ENext, nodeLabel e)} \<subseteq> F;
-      static_flow_set V F may_be_recv_site e
-    \<rbrakk> \<Longrightarrow>
-    static_flow_set V F may_be_recv_site (LET x = SEND EVT x\<^sub>c x\<^sub>m in e)
-  " |
-  Let_Recv_Evt: "
-    \<lbrakk>
-      {(NLet x, ENext, nodeLabel e)} \<subseteq> F;
-      static_flow_set V F may_be_recv_site e
-    \<rbrakk> \<Longrightarrow>
-    static_flow_set V F may_be_recv_site (LET x = RECV EVT x\<^sub>c in e)
-  " |
-  Let_Pair: "
-    \<lbrakk>
-      {(NLet x, ENext, nodeLabel e)} \<subseteq> F;
-      static_flow_set V F may_be_recv_site e
-    \<rbrakk> \<Longrightarrow>
-    static_flow_set V F may_be_recv_site (LET x = \<lparr>x\<^sub>1, x\<^sub>2\<rparr> in e)
-  " |
-  Let_Left: "
-    \<lbrakk>
-      {(NLet x, ENext, nodeLabel e)} \<subseteq> F;
-      static_flow_set V F may_be_recv_site e
-    \<rbrakk> \<Longrightarrow>
-    static_flow_set V F may_be_recv_site (LET x = LEFT x\<^sub>p in e)
-  " |
-  Let_Right: "
-    \<lbrakk>
-      {(NLet x, ENext, nodeLabel e)} \<subseteq> F;
-      static_flow_set V F may_be_recv_site e
-    \<rbrakk> \<Longrightarrow>
-    static_flow_set V F may_be_recv_site (LET x = RIGHT x\<^sub>p in e)
-  " |
-  Let_Abs: "
-    \<lbrakk>
-      {(NLet x, ENext, nodeLabel e)} \<subseteq> F;
-      static_flow_set V F may_be_recv_site e\<^sub>b;
-      static_flow_set V F may_be_recv_site e
-    \<rbrakk> \<Longrightarrow>
-    static_flow_set V F may_be_recv_site (LET x = FN f x\<^sub>p . e\<^sub>b  in e)
-  " |
-  Let_Spawn: "
-    \<lbrakk>
-      {
-        (NLet x, ENext, nodeLabel e),
-        (NLet x, ESpawn, nodeLabel e\<^sub>c)
-      } \<subseteq> F;
-      static_flow_set V F may_be_recv_site e\<^sub>c;
-      static_flow_set V F may_be_recv_site e
-    \<rbrakk> \<Longrightarrow>
-    static_flow_set V F may_be_recv_site (LET x = SPAWN e\<^sub>c in e)
-  " |
-  Let_Sync: "
-    \<lbrakk>
-      {(NLet x, ENext, nodeLabel e)} \<subseteq> F;
-      (\<forall> xSC xM xC y.
-        {^Send_Evt xSC xM} \<subseteq> V xSE \<longrightarrow>
-        {^Chan xC} \<subseteq> V xSC \<longrightarrow>
-        may_be_recv_site xC (NLet y) \<longrightarrow>
-        {(NLet x, ESend xSE, NLet y)} \<subseteq> F
-      );
-      static_flow_set V F may_be_recv_site e
-    \<rbrakk> \<Longrightarrow>
-    static_flow_set V F may_be_recv_site (LET x = SYNC xSE in e)
-  " |
-  Let_Fst: "
-    \<lbrakk>
-      {(NLet x, ENext, nodeLabel e)} \<subseteq> F;
-      static_flow_set V F may_be_recv_site e
-    \<rbrakk> \<Longrightarrow>
-    static_flow_set V F may_be_recv_site (LET x = FST x\<^sub>p in e)
-  " |
-  Let_Snd: "
-    \<lbrakk>
-      {(NLet x, ENext, nodeLabel e)} \<subseteq> F;
-      static_flow_set V F may_be_recv_site e
-    \<rbrakk> \<Longrightarrow>
-    static_flow_set V F may_be_recv_site (LET x = SND x\<^sub>p in e)
-  " |
-  Let_Case: "
-    \<lbrakk>
-      {
-        (NLet x, ECall x, nodeLabel e\<^sub>l),
-        (NLet x, ECall x, nodeLabel e\<^sub>r),
-        (NResult (\<lfloor>e\<^sub>l\<rfloor>), EReturn x, nodeLabel e),
-        (NResult (\<lfloor>e\<^sub>r\<rfloor>), EReturn x, nodeLabel e)
-      } \<subseteq> F;
-      static_flow_set V F may_be_recv_site e\<^sub>l;
-      static_flow_set V F may_be_recv_site e\<^sub>r;
-      static_flow_set V F may_be_recv_site e
-    \<rbrakk> \<Longrightarrow>
-    static_flow_set V F may_be_recv_site (LET x = CASE x\<^sub>s LEFT x\<^sub>l |> e\<^sub>l RIGHT x\<^sub>r |> e\<^sub>r in e)
-  " |
-  Let_App: "
-    \<lbrakk>
-      (\<forall> f' x\<^sub>p e\<^sub>b . ^Abs f' x\<^sub>p e\<^sub>b \<in> V f \<longrightarrow>
-        {
-          (NLet x, ECall x, nodeLabel e\<^sub>b),
-          (NResult (\<lfloor>e\<^sub>b\<rfloor>), EReturn x, nodeLabel e)
-        } \<subseteq> F);
-      static_flow_set V F may_be_recv_site e
-    \<rbrakk> \<Longrightarrow>
-    static_flow_set V F may_be_recv_site (LET x = APP f x\<^sub>a in e)
-  "
-
-inductive 
-  may_be_built_on_abstract_chan :: "abstract_value_env \<Rightarrow> node_map \<Rightarrow> var \<Rightarrow> var \<Rightarrow> bool"
-where
-  Chan: "
-    \<lbrakk>
-      ^Chan x\<^sub>c \<in> V x 
-    \<rbrakk> \<Longrightarrow> 
-    may_be_built_on_abstract_chan V Ln x\<^sub>c x
-  " |
-  Send_Evt: "
-    \<lbrakk>
-      ^Send_Evt x\<^sub>s\<^sub>c x\<^sub>m \<in> V x;
-      may_be_built_on_abstract_chan V Ln x\<^sub>c x\<^sub>s\<^sub>c \<or> may_be_built_on_abstract_chan V Ln x\<^sub>c x\<^sub>m 
-    \<rbrakk> \<Longrightarrow> 
-    may_be_built_on_abstract_chan V Ln x\<^sub>c x
-  " |
-  Recv_Evt: "
-    \<lbrakk>
-      ^Recv_Evt x\<^sub>r\<^sub>c \<in> V x;
-      may_be_built_on_abstract_chan V Ln x\<^sub>c x\<^sub>r\<^sub>c
-    \<rbrakk> \<Longrightarrow> 
-    may_be_built_on_abstract_chan V Ln x\<^sub>c x
-  " |
-  Pair: "
-    \<lbrakk>
-      ^(Pair x\<^sub>1 x\<^sub>2) \<in> V x;
-      may_be_built_on_abstract_chan V Ln x\<^sub>c x\<^sub>1 \<or> may_be_built_on_abstract_chan V Ln x\<^sub>c x\<^sub>2
-    \<rbrakk> \<Longrightarrow> 
-    may_be_built_on_abstract_chan V Ln x\<^sub>c x
-  " |
-  Left: "
-    \<lbrakk>
-      ^(Left x\<^sub>a) \<in> V x;
-      may_be_built_on_abstract_chan V Ln x\<^sub>c x\<^sub>a
-    \<rbrakk> \<Longrightarrow> 
-    may_be_built_on_abstract_chan V Ln x\<^sub>c x
-  " |
-  Right: "
-    \<lbrakk>
-      ^(Right x\<^sub>a) \<in> V x;
-      may_be_built_on_abstract_chan V Ln x\<^sub>c x\<^sub>a
-    \<rbrakk> \<Longrightarrow> 
-    may_be_built_on_abstract_chan V Ln x\<^sub>c x
-  " |
-  Abs: "
-    ^Abs f x\<^sub>p e\<^sub>b \<in> V x \<Longrightarrow> 
-    \<not> Set.is_empty (Ln (nodeLabel e\<^sub>b) - {x\<^sub>p}) \<Longrightarrow>
-    may_be_built_on_abstract_chan V Ln x\<^sub>c x
-  " 
-(*
-  |
-
-  Result: "
-    may_be_built_on_abstract_chan V Ln x\<^sub>c x \<Longrightarrow>
-    may_be_built_on_abstract_chan_exp V x\<^sub>c (RESULT x)
-  " |
-  Let: "
-    may_be_built_on_abstract_chan V Ln x\<^sub>c x \<or> 
-    may_be_built_on_abstract_chan_exp V x\<^sub>c e \<Longrightarrow>
-    may_be_built_on_abstract_chan_exp V x\<^sub>c (LET x = b in e)
-  "
-*)
-
-fun chan_set :: "abstract_value_env \<Rightarrow> node_map \<Rightarrow> var \<Rightarrow> var \<Rightarrow> var set" where
-  "chan_set V Ln x\<^sub>c x = (if (may_be_built_on_abstract_chan V Ln x\<^sub>c x) then {x} else {})"
-
-
-inductive static_chan_liveness :: "abstract_value_env \<Rightarrow> node_map \<Rightarrow> node_map \<Rightarrow> var \<Rightarrow> exp \<Rightarrow> bool" where
-  Result: "
-    \<lbrakk>
-      chan_set V Ln x\<^sub>c y = Ln (NResult y)
-    \<rbrakk> \<Longrightarrow>
-    static_chan_liveness V Ln Lx x\<^sub>c (RESULT y)
-  " |
-  Let_Unit: "
-    \<lbrakk>
-      static_chan_liveness V Ln Lx x\<^sub>c e;
-      Ln (nodeLabel e) = Lx (NLet x);
-      Lx (NLet x) = Ln (NLet x)
-    \<rbrakk> \<Longrightarrow>
-    static_chan_liveness V Ln Lx x\<^sub>c (LET x = \<lparr>\<rparr> in e)
-  " |
-  Let_Chan: "
-    \<lbrakk>
-      static_chan_liveness V Ln Lx x\<^sub>c e;
-      Ln (nodeLabel e) = Lx (NLet x);
-      (Lx (NLet x) - {x}) = Ln (NLet x)
-    \<rbrakk> \<Longrightarrow>
-    static_chan_liveness V Ln Lx x\<^sub>c (LET x = CHAN \<lparr>\<rparr> in e)
-  " |
-  Let_Send_Evt: "
-    \<lbrakk>
-      static_chan_liveness V Ln Lx x\<^sub>c e;
-      Ln (nodeLabel e) = Lx (NLet x);
-      (Lx (NLet x) - {x}) \<union> chan_set V Ln x\<^sub>c x\<^sub>s\<^sub>c \<union> chan_set V Ln x\<^sub>c x\<^sub>m = Ln (NLet x)
-    \<rbrakk> \<Longrightarrow>
-    static_chan_liveness V Ln Lx x\<^sub>c (LET x = SEND EVT x\<^sub>s\<^sub>c x\<^sub>m in e)
-  " |
-  Let_Recv_Evt: "
-    \<lbrakk>
-      static_chan_liveness V Ln Lx x\<^sub>c e;
-      Ln (nodeLabel e) = Lx (NLet x);
-      (Lx (NLet x) - {x}) \<union> chan_set V Ln x\<^sub>c x\<^sub>r\<^sub>c = Ln (NLet x)
-    \<rbrakk> \<Longrightarrow>
-    static_chan_liveness V Ln Lx x\<^sub>c (LET x = RECV EVT x\<^sub>r\<^sub>c in e)
-  " |
-  Let_Pair: "
-    \<lbrakk>
-      static_chan_liveness V Ln Lx x\<^sub>c e;
-      Ln (nodeLabel e) = Lx (NLet x);
-      (Lx (NLet x) - {x}) \<union>  chan_set V Ln x\<^sub>c x\<^sub>1 \<union> chan_set V Ln x\<^sub>c x\<^sub>2 = Ln (NLet x)
-    \<rbrakk> \<Longrightarrow>
-    static_chan_liveness V Ln Lx x\<^sub>c (LET x = \<lparr>x\<^sub>1, x\<^sub>2\<rparr> in e)
-  " |
-  Let_Left: "
-    \<lbrakk>
-      static_chan_liveness V Ln Lx x\<^sub>c e;
-      Ln (nodeLabel e) = Lx (NLet x);
-      (Lx (NLet x) - {x}) \<union> chan_set V Ln x\<^sub>c x\<^sub>a = Ln (NLet x)
-    \<rbrakk> \<Longrightarrow>
-    static_chan_liveness V Ln Lx x\<^sub>c (LET x = LEFT x\<^sub>a in e)
-  " |
-  Let_Right: "
-    \<lbrakk>
-      static_chan_liveness V Ln Lx x\<^sub>c e;
-      Ln (nodeLabel e) = Lx (NLet x);
-      (Lx (NLet x) - {x}) \<union> chan_set V Ln x\<^sub>c x\<^sub>a = Ln (NLet x)
-    \<rbrakk> \<Longrightarrow>
-    static_chan_liveness V Ln Lx x\<^sub>c (LET x = RIGHT x\<^sub>a in e)
-  " |
-  Let_Abs: "
-    \<lbrakk>
-      static_chan_liveness V Ln Lx x\<^sub>c e;
-      Ln (nodeLabel e) = Lx (NLet x);
-      static_chan_liveness V Ln Lx x\<^sub>c e\<^sub>b;
-      (Lx (NLet x) - {x}) \<union> (Ln (nodeLabel e\<^sub>b) - {x\<^sub>p}) = Ln (NLet x)
-    \<rbrakk> \<Longrightarrow>
-    static_chan_liveness V Ln Lx x\<^sub>c (LET x = FN f x\<^sub>p . e\<^sub>b  in e)
-  " |
-  Let_Spawn: "
-    \<lbrakk>
-      static_chan_liveness V Ln Lx x\<^sub>c e;
-      static_chan_liveness V Ln Lx x\<^sub>c e\<^sub>c;
-      Ln (nodeLabel e) \<union> Ln (nodeLabel e\<^sub>c) = Lx (NLet x);
-      (Lx (NLet x) - {x}) = Ln (NLet x)
-    \<rbrakk> \<Longrightarrow>
-    static_chan_liveness V Ln Lx x\<^sub>c (LET x = SPAWN e\<^sub>c in e)
-  " |
-  Let_Sync: "
-    \<lbrakk>
-      static_chan_liveness V Ln Lx x\<^sub>c e;
-      Ln (nodeLabel e) = Lx (NLet x);
-      (Lx (NLet x) - {x}) \<union> chan_set V Ln x\<^sub>c x\<^sub>e = Ln (NLet x)
-    \<rbrakk> \<Longrightarrow>
-    static_chan_liveness V Ln Lx x\<^sub>c (LET x = SYNC x\<^sub>e in e)
-  " |
-  Let_Fst: "
-    \<lbrakk>
-      static_chan_liveness V Ln Lx x\<^sub>c e;
-      Ln (nodeLabel e) = Lx (NLet x);
-      (Lx (NLet x) - {x}) \<union> chan_set V Ln x\<^sub>c x\<^sub>a = Ln (NLet x)
-    \<rbrakk> \<Longrightarrow>
-    static_chan_liveness V Ln Lx x\<^sub>c (LET x = FST x\<^sub>a in e)
-  " |
-  Let_Snd: "
-    \<lbrakk>
-      static_chan_liveness V Ln Lx x\<^sub>c e;
-      Ln (nodeLabel e) = Lx (NLet x);
-      (Lx (NLet x) - {x}) \<union> chan_set V Ln x\<^sub>c x\<^sub>a = Ln (NLet x)
-    \<rbrakk> \<Longrightarrow>
-    static_chan_liveness V Ln Lx x\<^sub>c (LET x = SND x\<^sub>a in e)
-  " |
-  Let_Case: "
-    \<lbrakk>
-      static_chan_liveness V Ln Lx x\<^sub>c e;
-      Ln (nodeLabel e) = Lx (NLet x);
-      static_chan_liveness V Ln Lx x\<^sub>c e\<^sub>l;
-      static_chan_liveness V Ln Lx x\<^sub>c e\<^sub>r;
-      (Lx (NLet x) - {x}) \<union> chan_set V Ln x\<^sub>c x\<^sub>s \<union> 
-         (Ln (nodeLabel e\<^sub>l) - {x\<^sub>l}) \<union> (Ln (nodeLabel e\<^sub>r) - {x\<^sub>r}) = Ln (NLet x)
-    \<rbrakk> \<Longrightarrow>
-    static_chan_liveness V Ln Lx x\<^sub>c (LET x = CASE x\<^sub>s LEFT x\<^sub>l |> e\<^sub>l RIGHT x\<^sub>r |> e\<^sub>r in e)
-  " |
-  Let_App: "
-    \<lbrakk>
-      static_chan_liveness V Ln Lx x\<^sub>c e;
-      Ln (nodeLabel e) = Lx (NLet x);
-      (Lx (NLet x) - {x}) \<union> chan_set V Ln x\<^sub>c f \<union> chan_set V Ln x\<^sub>c x\<^sub>a = Ln (NLet x)
-    \<rbrakk> \<Longrightarrow>
-    static_chan_liveness V Ln Lx x\<^sub>c (LET x = APP f x\<^sub>a in e)
-  "
-
-
-
-
-inductive may_be_static_path :: "flow_set \<Rightarrow> node_label \<Rightarrow> static_path \<Rightarrow> bool" where
-  Empty: "
-    may_be_static_path F end []
-  " |
-  Edge: "
-    (start, edge, end) \<in> F \<Longrightarrow>
-    may_be_static_path F end [(start, edge)]
-  " |
-  Step: "
-    may_be_static_path F end ((middle, edge') # post) \<Longrightarrow>
-    (start, edge, middle) \<in> F \<Longrightarrow>
-    path = [(start, edge), (middle, edge')] @ post \<Longrightarrow>
-    may_be_static_path F end path
-  "
-
-inductive static_balanced :: "static_path \<Rightarrow> bool" where
-  Empty: "
-    static_balanced []
-  " |
-  Next: "
-    static_balanced [(NLet x, ENext)]
-  " |
-  CallReturn: "
-    static_balanced path \<Longrightarrow>
-    static_balanced ((NLet x, ECall x) # (path @ [(NResult y, EReturn x)]))
-  " |
-  Append: "
-    path \<noteq> [] \<Longrightarrow>
-    static_balanced path \<Longrightarrow>
-    path' \<noteq> [] \<Longrightarrow>
-    static_balanced path' \<Longrightarrow>
-    static_balanced (path @ path')
-  "
-
-inductive static_unbalanced :: "static_path \<Rightarrow> bool" where
-  Result: "
-    static_unbalanced ((NResult y, EReturn x) # post)
-  " |
-  Next: "
-    static_unbalanced post \<Longrightarrow>
-    static_unbalanced ((NLet x, ENext) # post)
-  "
-
-
-inductive may_be_static_live_flow :: "flow_set \<Rightarrow> node_map \<Rightarrow> node_map \<Rightarrow> flow_label \<Rightarrow> bool"  where
-  Next: "
-    (l, ENext, l') \<in> F \<Longrightarrow>
-    \<not> Set.is_empty (Lx l) \<Longrightarrow>
-    \<not> Set.is_empty (Ln l') \<Longrightarrow>
-    may_be_static_live_flow F Ln Lx (l, ENext, l')
-  " |
-  Spawn: "
-    (l, ESpawn, l') \<in> F \<Longrightarrow>
-    \<not> Set.is_empty (Lx l) \<Longrightarrow>
-    \<not> Set.is_empty (Ln l') \<Longrightarrow>
-    may_be_static_live_flow F Ln Lx (l, ESpawn, l')
-  " |
-  Call_Live_Outer: "
-    (l, ECall x, l') \<in> F \<Longrightarrow>
-    \<not> Set.is_empty (Lx l) \<Longrightarrow>
-    may_be_static_live_flow F Ln Lx (l, ECall x, l')
-  " |
-  Call_Live_Inner: "
-    (l, ECall x, l') \<in> F \<Longrightarrow>
-    \<not> Set.is_empty (Ln l') \<Longrightarrow>
-    may_be_static_live_flow F Ln Lx (l, ECall x, l')
-  " |
-  Return: "
-    (l, EReturn x, l') \<in> F \<Longrightarrow>
-    \<not> Set.is_empty (Ln l') \<Longrightarrow>
-    may_be_static_live_flow F Ln Lx (l, EReturn x, l')
-  " |
-  Send: "
-    ((NLet xSend), ESend xE, (NLet xRecv)) \<in> F \<Longrightarrow>
-    {xE} \<subseteq> (Ln (NLet xSend)) \<Longrightarrow>
-    may_be_static_live_flow F Ln Lx ((NLet xSend), ESend xE, (NLet xRecv))
-  "
-
-inductive may_be_static_live_path :: "abstract_value_env \<Rightarrow> flow_set \<Rightarrow> node_map \<Rightarrow> node_map \<Rightarrow> node_label \<Rightarrow> (node_label \<Rightarrow> bool) \<Rightarrow> static_path \<Rightarrow> bool" where
-  Empty: "
-    isEnd start \<Longrightarrow>
-    may_be_static_live_path V F Ln Lx start isEnd []
-  " |
-  Edge: "
-    isEnd end \<Longrightarrow>
-    may_be_static_live_flow F Ln Lx (start, edge, end) \<Longrightarrow>
-    may_be_static_live_path V F Ln Lx start isEnd [(start, edge)]
-  " |
-  Step: "
-    may_be_static_live_path V F Ln Lx middle isEnd ((middle, edge') # path) \<Longrightarrow>
-    may_be_static_live_flow F Ln Lx (start, edge, middle) \<Longrightarrow>
-    may_be_static_live_path V F Ln Lx start isEnd ((start, edge) # (middle, edge') # path)
-  " |
-
-  Pre_Return: "
-    may_be_static_live_path V F Ln Lx (NResult y) isEnd ((NResult y, EReturn x) # post) \<Longrightarrow>
-    may_be_static_path  F (NResult y) pre \<Longrightarrow>
-    \<not> static_balanced (pre @ [(NResult y, EReturn x)]) \<Longrightarrow>
-    \<not> Set.is_empty (Lx (NLet x)) \<Longrightarrow>
-    path = pre @ (NResult y, EReturn x) # post \<Longrightarrow>
-    may_be_static_live_path V F Ln Lx start isEnd path
-  "
-
-
-inductive may_be_inclusive :: "static_path \<Rightarrow> static_path \<Rightarrow> bool" (infix "\<asymp>" 55) where
-  Prefix1: "
-    prefix \<pi>\<^sub>1 \<pi>\<^sub>2 \<Longrightarrow>
-    \<pi>\<^sub>1 \<asymp> \<pi>\<^sub>2
-  " |
-  Prefix2: "
-    prefix \<pi>\<^sub>2 \<pi>\<^sub>1 \<Longrightarrow>
-    \<pi>\<^sub>1 \<asymp> \<pi>\<^sub>2
-  " |
-  Spawn1: "
-    \<pi> @ (NLet x, ESpawn) # \<pi>\<^sub>1 \<asymp> \<pi> @ (NLet x, ENext) # \<pi>\<^sub>2
-  " |
-  Spawn2: "
-    \<pi> @ (NLet x, ENext) # \<pi>\<^sub>1 \<asymp> \<pi> @ (NLet x, ESpawn) # \<pi>\<^sub>2
-  " |
-  Send1: "
-    \<pi> @ (NLet x, ESend xE) # \<pi>\<^sub>1 \<asymp> \<pi> @ (NLet x, ENext) # \<pi>\<^sub>2
-  " |
-  Send2: "
-    \<pi> @ (NLet x, ENext) # \<pi>\<^sub>1 \<asymp> \<pi> @ (NLet x, ESend xE) # \<pi>\<^sub>2
-  " |
-  Kite: "
-    p1 @ [(NLet x1, ESend xE1)] \<noteq> (p2 @ [(NLet x2, ESend xE2)]) \<Longrightarrow>
-    ((NLet x, ENext) # p1 @ [(NLet x1, ESend xE1)] @ p1') \<asymp> 
-      ((NLet x, ENext) # p2 @ [(NLet x2, ESend xE2)] @ p2')
-  "
-
-lemma may_be_inclusive_commut: "
-  path\<^sub>1 \<asymp> path\<^sub>2 \<Longrightarrow> path\<^sub>2 \<asymp> path\<^sub>1
-"
- apply (erule may_be_inclusive.cases; auto)
-  apply (simp add: Prefix2)
-  apply (simp add: Prefix1)
-  apply (simp add: Spawn2)
-  apply (simp add: Spawn1)
-  apply (simp add: Send2)
-  apply (simp add: Send1)
-  using Kite apply auto[1]
-  using Kite apply auto[1]
-  using Kite apply auto[1]
-done
-
-
-lemma may_be_inclusive_preserved_under_unordered_extension: "
-  \<not> prefix path\<^sub>1 path\<^sub>2 \<Longrightarrow> \<not> prefix path\<^sub>2 path\<^sub>1 \<Longrightarrow> path\<^sub>1 \<asymp> path\<^sub>2 \<Longrightarrow> path\<^sub>1 @ [l] \<asymp> path\<^sub>2
-"
- apply (erule may_be_inclusive.cases; auto)
-  apply (simp add: Spawn1)
-  apply (simp add: Spawn2)
-  apply (simp add: Send1)
-  apply (simp add: Send2)
-  using Kite apply auto[1]
-  using Kite apply auto[1]
-  using Kite apply auto
-done
-
-lemma may_be_inclusive_preserved_under_unordered_double_extension: "
-  path\<^sub>1 \<asymp> path\<^sub>2 \<Longrightarrow> \<not> prefix path\<^sub>1 path\<^sub>2 \<Longrightarrow> \<not> prefix path\<^sub>2 path\<^sub>1 \<Longrightarrow> path\<^sub>1 @ [l1] \<asymp> path\<^sub>2 @ [l2]
-"
-by (metis may_be_inclusive_commut may_be_inclusive_preserved_under_unordered_extension prefix_append prefix_def)
-
-inductive singular :: "static_path \<Rightarrow> static_path \<Rightarrow> bool" where
-  equal: "
-    \<pi>\<^sub>1 = \<pi>\<^sub>2 \<Longrightarrow> 
-    singular \<pi>\<^sub>1 \<pi>\<^sub>2
-  " |
-  exclusive: "
-    \<not> (\<pi>\<^sub>1 \<asymp> \<pi>\<^sub>2) \<Longrightarrow> 
-    singular \<pi>\<^sub>1 \<pi>\<^sub>2
-  "
-
-inductive noncompetitive :: "static_path \<Rightarrow> static_path \<Rightarrow> bool" where
-  ordered: "
-    ordered \<pi>\<^sub>1 \<pi>\<^sub>2 \<Longrightarrow> 
-    noncompetitive \<pi>\<^sub>1 \<pi>\<^sub>2
-  " |
-  exclusive: "
-    \<not> (\<pi>\<^sub>1 \<asymp> \<pi>\<^sub>2) \<Longrightarrow> 
-    noncompetitive \<pi>\<^sub>1 \<pi>\<^sub>2
-  "
-
-
-inductive every_two_static_paths  :: "(static_path \<Rightarrow> bool) \<Rightarrow> (static_path \<Rightarrow> static_path \<Rightarrow> bool) \<Rightarrow> bool" where
-  pred: "
-    (\<forall> path1 path2 . P path1 \<longrightarrow> P path2 \<longrightarrow> 
-      R path1 path2) \<Longrightarrow>
-    every_two_static_paths P R
-  "
-
-
-inductive static_one_shot :: "abstract_value_env \<Rightarrow> exp \<Rightarrow> var \<Rightarrow> bool" where
-  Sync: "
-    every_two_static_paths (may_be_static_live_path V F Ln Lx (NLet xC) (may_be_static_send_node_label V e xC)) singular \<Longrightarrow>
-    static_chan_liveness V Ln Lx xC e \<Longrightarrow>
-    static_flow_set V F (may_be_static_recv_node_label V e) e \<Longrightarrow>
-    static_one_shot V e xC 
-  "
-
-inductive static_one_to_one :: "abstract_value_env \<Rightarrow> exp \<Rightarrow> var \<Rightarrow> bool" where
-  Sync: "
-    every_two_static_paths (may_be_static_live_path V F Ln Lx (NLet xC) (may_be_static_send_node_label V e xC)) noncompetitive \<Longrightarrow>
-    every_two_static_paths (may_be_static_live_path V F Ln Lx (NLet xC) (may_be_static_recv_node_label V e xC)) noncompetitive \<Longrightarrow>
-    static_chan_liveness V Ln Lx xC e \<Longrightarrow>
-    static_flow_set V F (may_be_static_recv_node_label V e) e \<Longrightarrow>
-    static_one_to_one V e xC 
-  "
-
-inductive static_fan_out :: "abstract_value_env \<Rightarrow> exp \<Rightarrow> var \<Rightarrow> bool" where
-  Sync: "
-    every_two_static_paths (may_be_static_live_path V F Ln Lx (NLet xC) (may_be_static_send_node_label V e xC)) noncompetitive \<Longrightarrow>
-    static_chan_liveness V Ln Lx xC e \<Longrightarrow>
-    static_flow_set V F (may_be_static_recv_node_label V e) e \<Longrightarrow>
-    static_fan_out V e xC 
-  "
-
-inductive static_fan_in :: "abstract_value_env \<Rightarrow> exp \<Rightarrow> var \<Rightarrow> bool" where
-  Sync: "
-    every_two_static_paths (may_be_static_live_path V F Ln Lx (NLet xC) (may_be_static_recv_node_label V e xC)) noncompetitive \<Longrightarrow>
-    static_chan_liveness V Ln Lx xC e \<Longrightarrow>
-    static_flow_set V F (may_be_static_recv_node_label V e) e \<Longrightarrow>
-    static_fan_in V e xC 
-  "
-
-
-
-inductive 
-  dynamic_built_on_chan_var :: "(var \<rightharpoonup> val) \<Rightarrow> chan \<Rightarrow> var \<Rightarrow> bool" and
-  dynamic_built_on_chan_prim :: "(var \<rightharpoonup> val) \<Rightarrow> chan \<Rightarrow> prim \<Rightarrow> bool" and
-  dynamic_built_on_chan_bindee :: "(var \<rightharpoonup> val) \<Rightarrow> chan \<Rightarrow> bind \<Rightarrow> bool" and
-  dynamic_built_on_chan_exp :: "(var \<rightharpoonup> val) \<Rightarrow> chan \<Rightarrow> exp \<Rightarrow> bool" 
-where
-  Chan: "
-    \<rho> x = Some (VChan c) \<Longrightarrow>
-    dynamic_built_on_chan_var \<rho> c x
-  " |
-  Closure: "
-    dynamic_built_on_chan_prim \<rho>' c p \<Longrightarrow>
-    \<rho> x = Some (VClosure p \<rho>') \<Longrightarrow>
-    dynamic_built_on_chan_var \<rho> c x
-  " |
-
-
-  Send_Evt: "
-    dynamic_built_on_chan_var \<rho> c xSC \<or> dynamic_built_on_chan_var \<rho> c xM \<Longrightarrow>
-    dynamic_built_on_chan_prim \<rho> c (Send_Evt xSC xM)
-  " |
-  Recv_Evt: "
-    dynamic_built_on_chan_var \<rho> c xRC \<Longrightarrow>
-    dynamic_built_on_chan_prim \<rho> c (Recv_Evt xRC)
-  " |
-  Pair: "
-    dynamic_built_on_chan_var \<rho> c x1 \<or> dynamic_built_on_chan \<rho> c x2 \<Longrightarrow>
-    dynamic_built_on_chan_prim \<rho> c (Pair x1 x2)
-  " |
-  Left: "
-    dynamic_built_on_chan_var \<rho> c xSum \<Longrightarrow>
-    dynamic_built_on_chan_prim \<rho> c (Left xSum)
-  " |
-  Right: "
-    dynamic_built_on_chan_var \<rho> c xSum \<Longrightarrow>
-    dynamic_built_on_chan_prim \<rho> c (Right xSum)
-  " |
-  Abs: "
-    dynamic_built_on_chan_exp \<rho>' c e \<Longrightarrow>
-    dynamic_built_on_chan_prim \<rho> c (Abs f x e)
-  " |
-
-  Prim: "
-    dynamic_built_on_chan_prim \<rho> c p \<Longrightarrow>
-    dynamic_built_on_chan_bindee \<rho> c (Prim p)
-  " |
-  Spawn: "
-    dynamic_built_on_chan_exp \<rho> c eCh \<Longrightarrow>
-    dynamic_built_on_chan_bindee \<rho> c (SPAWN eCh)
-  " |
-  Sync: "
-    dynamic_built_on_chan_var \<rho> c xY \<Longrightarrow>
-    dynamic_built_on_chan_bindee \<rho> c (SYNC xY)
-  " |
-  Fst: "
-    dynamic_built_on_chan_var \<rho> c xP \<Longrightarrow>
-    dynamic_built_on_chan_bindee \<rho> c (FST xP)
-  " |
-  Snd: "
-    dynamic_built_on_chan_var \<rho> c xP \<Longrightarrow>
-    dynamic_built_on_chan_bindee \<rho> c (SND xP)
-  " |
-  Case: "
-    dynamic_built_on_chan_var \<rho> c xS \<or> 
-    dynamic_built_on_chan_exp \<rho> c eL \<or> dynamic_built_on_chan_exp \<rho> c eR \<Longrightarrow>
-    dynamic_built_on_chan_bindee \<rho> c (CASE xS LEFT xL |> eL RIGHT xR |> eR)
-  " |
-  App: "
-    dynamic_built_on_chan_var \<rho> c f \<or>
-    dynamic_built_on_chan_var \<rho> c xA \<Longrightarrow>
-    dynamic_built_on_chan_bindee \<rho> c (APP f xA)
-  " |
-
-  Result: "
-    dynamic_built_on_chan_var \<rho> c x \<Longrightarrow>
-    dynamic_built_on_chan_exp \<rho> c (RESULT x)
-  " |
-  Let: "
-    dynamic_built_on_chan_bindee \<rho> c b \<or> dynamic_built_on_chan_exp \<rho> c e \<Longrightarrow>
-    dynamic_built_on_chan_exp \<rho> c (LET x = b in e)
-  "
-
-
-inductive nodes_congruent :: "control_label \<Rightarrow> step_label \<Rightarrow> bool" where
-  Next: "
-    nodes_congruent (LNext x) (NLet x, ENext)" |
-  Call: "
-    nodes_congruent (LCall x) (NLet x, ECall x)" |
-  Return: "
-    nodes_congruent (LReturn y) (NResult y, EReturn x)" |
-  Spawn: "
-    nodes_congruent (LSpawn x) (NLet x, ESpawn)"
-
-
-inductive paths_congruent :: "control_path \<Rightarrow> static_path \<Rightarrow> bool" where
-  Node: "
-    paths_congruent [] []
-  " |
-  List: "
-    nodes_congruent l n \<Longrightarrow>
-    paths_congruent \<pi> path \<Longrightarrow>
-    paths_congruent (\<pi> ;; l) (path @ [n])
-  "
-
-inductive paths_congruent_mod_chan :: "trace_pool * com_set \<Rightarrow> chan \<Rightarrow> control_path \<Rightarrow> static_path \<Rightarrow> bool" where
-  Unordered: "
-    paths_congruent \<pi> pathx \<Longrightarrow>
-    \<not> (prefix pathx path) \<Longrightarrow>
-    \<not> (prefix path pathx) \<Longrightarrow>
-    paths_congruent_mod_chan (\<E>, H) c \<pi> path
-  " |
-  Chan: "
-    paths_congruent ((LNext xC) # \<pi>Suff) path \<Longrightarrow>
-    \<E> (\<pi>C @ (LNext xC) # \<pi>Suff) \<noteq> None \<Longrightarrow>
-    paths_congruent_mod_chan (\<E>, H) (Ch \<pi>C xC) (\<pi>C @ (LNext xC) # \<pi>Suff) path
-  " |
-  Sync: "
-    paths_congruent \<pi>Suffix pathSuffix \<Longrightarrow>
-    \<E> (\<pi>R @ (LNext xR) # \<pi>Suffix) \<noteq> None \<Longrightarrow>
-    dynamic_built_on_chan_var \<rho>RY c xR \<Longrightarrow>
-    \<E> \<pi>S = Some (\<langle>LET xS = SYNC xSE in eSY;\<rho>SY;\<kappa>SY\<rangle>) \<Longrightarrow>
-    \<E> \<pi>R = Some (\<langle>LET xR = SYNC xRE in eRY;\<rho>RY;\<kappa>RY\<rangle>) \<Longrightarrow>
-    {(\<pi>S, c, \<pi>R)} \<subseteq> H \<Longrightarrow>
-    paths_congruent_mod_chan (\<E>, H) c \<pi>S pathPre \<Longrightarrow>
-    paths_congruent_mod_chan (\<E>, H) c (\<pi>R @ (LNext xR) # \<pi>Suffix) (pathPre @ (NLet xS, ESend xSE) # (NLet xR, ENext) # pathSuffix)
-  " 
-
-lemma no_empty_paths_congruent_mod_chan: "
-  \<not> (paths_congruent_mod_chan EH c [] path)"
-  apply (rule notI)
-  apply (erule paths_congruent_mod_chan.cases; auto)
-  apply (metis paths_congruent.simps prefix_code(1) snoc_eq_iff_butlast)
-done
-
-lemma static_paths_of_same_run_inclusive_base: "
+lemma abstract_paths_of_same_run_inclusive_base: "
   E0 = [[] \<mapsto> \<langle>e;Map.empty;[]\<rangle>] \<Longrightarrow>
   E0 \<pi>1 \<noteq> None \<Longrightarrow>
   E0 \<pi>2 \<noteq> None \<Longrightarrow>
@@ -1509,11 +726,6 @@ lemma paths_equal_implies_paths_inclusive: "
 "
 by (simp add: Prefix2)
 
-lemma paths_cong_preserved_under_reduction: "
-  paths_congruent (\<pi> ;; l) (path @ [n]) \<Longrightarrow>
-  paths_congruent \<pi> path"
-using paths_congruent.cases by fastforce
-
 
 lemma equal_concrete_paths_implies_unordered_or_equal_abstract_paths: "
 paths_congruent_mod_chan EH c \<pi> path1 \<Longrightarrow>
@@ -1522,31 +734,13 @@ path1 = path2 \<or> (\<not> prefix path1 path2 \<and> \<not> prefix path2 path1)
 "
 sorry
 
-lemma path_cong_mod_chan_preserved_under_reduction: "
+lemma paths_cong_mod_chan_preserved_under_reduction: "
 paths_congruent_mod_chan (E', H') (Ch \<pi>C xC) (\<pi> ;; l) (path @ [n]) \<Longrightarrow>
 (E, H) \<rightarrow> (E', H') \<Longrightarrow>
 paths_congruent_mod_chan (E, H) (Ch \<pi>C xC) \<pi> path
 "
 sorry
 
-(*
-lemma paths_cong_mod_chan_preserved_under_reduction_chan: "
-  paths_congruent ((LNext xC) # \<pi>Suff ;; l) (path @ [n]) \<Longrightarrow>
-  E (\<pi>C @ (LNext xC) # \<pi>Suff) \<noteq> None \<Longrightarrow>
-  paths_congruent_mod_chan (E, H) (Ch \<pi>C xC) (\<pi>C @ (LNext xC) # \<pi>Suff) path"
-using paths_cong_preserved_under_reduction paths_congruent_mod_chan.Chan by blast
-
-lemma  paths_cong_mod_chan_preserved_under_reduction_sync: "
-  paths_congruent (\<pi>Suffix ;; l) (pathSuffix @ [n]) \<Longrightarrow>
-  \<E> (\<pi>R @ (LNext xR) # \<pi>Suffix) \<noteq> None \<Longrightarrow>
-  dynamic_built_on_chan_var \<rho>RY c xR \<Longrightarrow>
-  \<E> \<pi>S = Some (\<langle>LET xS = SYNC xSE in eSY;\<rho>SY;\<kappa>SY\<rangle>) \<Longrightarrow>
-  \<E> \<pi>R = Some (\<langle>LET xR = SYNC xRE in eRY;\<rho>RY;\<kappa>RY\<rangle>) \<Longrightarrow>
-  {(\<pi>S, c, \<pi>R)} \<subseteq> H \<Longrightarrow>
-  paths_congruent_mod_chan (\<E>, H) c \<pi>S pathPre \<Longrightarrow>
-  paths_congruent_mod_chan (\<E>, H) c (\<pi>R @ (LNext xR) # \<pi>Suffix) (pathPre @ (NLet xS, ESend xSE) # (NLet xR, ENext) # pathSuffix)"
-by (meson paths_cong_preserved_under_reduction paths_congruent_mod_chan.Sync)
-*)
 
 lemma leaf_prefix_exists: "
   leaf E' (\<pi> ;; l) \<Longrightarrow>
@@ -1569,7 +763,7 @@ apply (erule concur_step.cases; auto; (erule seq_step.cases; auto)?)
 done
 
 
-lemma static_paths_of_same_run_inclusive_step: "
+lemma abstract_paths_of_same_run_inclusive_step: "
 \<forall>\<pi>1 \<pi>2 path1 path2.
   E \<pi>1 \<noteq> None \<longrightarrow>
   E \<pi>2 \<noteq> None \<longrightarrow>
@@ -1584,13 +778,6 @@ paths_congruent_mod_chan (E', H') (Ch \<pi>C xC) \<pi>1 path1 \<Longrightarrow>
 paths_congruent_mod_chan (E', H') (Ch \<pi>C xC) \<pi>2 path2 \<Longrightarrow>
 path1 \<asymp> path2 
 "
-(* TO DO: switch to ISAR style;
-
-   derive equal and unordered paths; 
-   derive inclusive paths
-
-*)
-
 proof ((case_tac "path1 = []"; (simp add: Prefix1)), (case_tac "path2 = []", (simp add: Prefix2)))
   assume 
     H1: "
@@ -1620,13 +807,13 @@ proof ((case_tac "path1 = []"; (simp add: Prefix1)), (case_tac "path2 = []", (si
     H12: "\<pi>1x ;; l1 = \<pi>1" and
     H13: "path1x @ [n1] = path1" and
     H14: "paths_congruent_mod_chan (E, H) (Ch \<pi>C xC) \<pi>1x path1x" 
-  by (metis H3 H6 H8 append_butlast_last_id path_cong_mod_chan_preserved_under_reduction no_empty_paths_congruent_mod_chan)
+  by (metis H3 H6 H8 append_butlast_last_id paths_cong_mod_chan_preserved_under_reduction no_empty_paths_congruent_mod_chan)
 
   obtain \<pi>2x l2 path2x n2 where
     H15: "\<pi>2x ;; l2 = \<pi>2" and
     H16: "path2x @ [n2] = path2" and
     H17: "paths_congruent_mod_chan (E, H) (Ch \<pi>C xC) \<pi>2x path2x"
-  by (metis H3 H7 H9 append_butlast_last_id path_cong_mod_chan_preserved_under_reduction no_empty_paths_congruent_mod_chan)
+  by (metis H3 H7 H9 append_butlast_last_id paths_cong_mod_chan_preserved_under_reduction no_empty_paths_congruent_mod_chan)
 
 
   have H18: "paths_congruent_mod_chan (E, H) (Ch \<pi>C xC) \<pi>1 path1" sorry
@@ -1645,7 +832,6 @@ proof ((case_tac "path1 = []"; (simp add: Prefix1)), (case_tac "path2 = []", (si
         L2H2: "E \<pi>2x = Some \<sigma>2x" using L2H1 leaf.simps by auto
       have "path1x \<asymp> path2x"
         using H1 H14 H17 L1H2 L2H2 by blast
-      (* inclusive definition fails in case of non-unique variable bindings *)
       show "path1 \<asymp> path2" sorry
     next
       assume L2H1: "\<not> leaf E \<pi>2x"
@@ -1700,23 +886,9 @@ proof ((case_tac "path1 = []"; (simp add: Prefix1)), (case_tac "path2 = []", (si
   qed
 
 qed
-(*
-apply ((case_tac "path1 = []"; (auto simp: Prefix1)), (case_tac "path2 = []", (auto simp: Prefix2)))
-apply (case_tac "path2 = []", (auto simp: Prefix2))
-apply (erule concur_step.cases; auto; (erule seq_step.cases; auto)?)
-  apply (case_tac "\<pi>1 = \<pi> ;; LReturn x\<^sub>\<kappa>"; auto; (case_tac "\<pi>2 = \<pi> ;; LReturn x\<^sub>\<kappa>"; auto)?)
-  apply (drule_tac x = \<pi> in spec; auto)
-  apply (drule_tac x = \<pi> in spec; auto)
-  apply (drule_tac x = "(butlast path1)" in spec; auto)
-  apply (metis append_butlast_last_id path_cong_mod_chan_preserved_under_reduction)
-  apply (drule_tac x = "(butlast path2)" in spec; auto)
-  apply (metis append_butlast_last_id path_cong_mod_chan_preserved_under_reduction)
-  apply (erule paths_congruent_mod_chan.cases; auto; (erule paths_congruent_mod_chan.cases; auto))
-  apply (erule paths_congruent.cases; auto; (erule paths_congruent.cases; auto); (erule nodes_congruent.cases))
-done
-*)
 
-lemma static_paths_of_same_run_inclusive: "
+
+lemma abstract_paths_of_same_run_inclusive: "
   ([[] \<mapsto> \<langle>e;Map.empty;[]\<rangle>], {}) \<rightarrow>* (\<E>', H') \<Longrightarrow> 
   \<E>' \<pi>1 \<noteq> None \<Longrightarrow> 
   \<E>' \<pi>2 \<noteq> None \<Longrightarrow> 
@@ -1753,7 +925,7 @@ proof -
   proof induction
     case (refl z)
     then show ?case
-      using static_paths_of_same_run_inclusive_base by blast
+      using abstract_paths_of_same_run_inclusive_base by blast
   next
     case (step x y z)
 
@@ -1782,7 +954,7 @@ proof -
 
       have 
         "path1 \<asymp> path2"
-        using L2H1 L2H2 L2H3 L2H4 L2H5 L2H6 L2H7 L2H8 static_paths_of_same_run_inclusive_step step.hyps(1) step.hyps(2) by blast
+        using L2H1 L2H2 L2H3 L2H4 L2H5 L2H6 L2H7 L2H8 abstract_paths_of_same_run_inclusive_step step.hyps(1) step.hyps(2) by blast
     }
     then show ?case by blast
   qed
@@ -1807,7 +979,7 @@ proof -
     "\<E> \<pi> \<noteq> None" by blast
 qed
 
-lemma send_static_paths_of_same_run_inclusive: "
+lemma send_abstract_paths_of_same_run_inclusive: "
   ([[] \<mapsto> \<langle>e;Map.empty;[]\<rangle>], {}) \<rightarrow>* (\<E>', H') \<Longrightarrow> 
   is_send_path \<E>' (Ch \<pi> xC) \<pi>1 \<Longrightarrow> 
   is_send_path \<E>' (Ch \<pi> xC) \<pi>2 \<Longrightarrow> 
@@ -1815,7 +987,8 @@ lemma send_static_paths_of_same_run_inclusive: "
   paths_congruent_mod_chan (\<E>', H') (Ch \<pi> xC) \<pi>2 path2 \<Longrightarrow>
   path1 \<asymp> path2
 "
-using is_send_path_implies_nonempty_pool static_paths_of_same_run_inclusive by fastforce
+using is_send_path_implies_nonempty_pool abstract_paths_of_same_run_inclusive by fastforce
+
 
 
 lemma send_path_equality_sound: "
@@ -1830,7 +1003,7 @@ lemma send_path_equality_sound: "
 sorry
 
 
-lemma send_static_paths_equal_exclusive_implies_dynamic_paths_equal: "
+lemma send_abstract_paths_equal_exclusive_implies_dynamic_paths_equal: "
 pathSync = pathSynca \<or> \<not> pathSync \<asymp> pathSynca \<Longrightarrow> 
 
 ([[] \<mapsto> \<langle>e;Map.empty;[]\<rangle>], {}) \<rightarrow>* (\<E>', H') \<Longrightarrow>
@@ -1842,9 +1015,7 @@ paths_congruent_mod_chan (\<E>', H') (Ch \<pi> xC) \<pi>\<^sub>2 pathSynca \<Lon
 
 \<pi>\<^sub>1 = \<pi>\<^sub>2
 "
-by (simp add: send_path_equality_sound send_static_paths_of_same_run_inclusive)
-
-(* END *)
+by (simp add: send_path_equality_sound send_abstract_paths_of_same_run_inclusive)
 
 (* PATH SOUND *)
 
@@ -1940,24 +1111,22 @@ done
 (* END PATH SOUND *)
 
 
-
 theorem one_shot_sound': "
-  every_two_static_paths (may_be_static_live_path V F Ln Lx (NLet xC) (may_be_static_send_node_label V e xC)) singular \<Longrightarrow>
+  every_two (may_be_static_live_path V F Ln Lx (NLet xC) (may_be_static_send_node_label V e xC)) singular \<Longrightarrow>
   static_chan_liveness V Ln Lx xC e \<Longrightarrow>
   static_flow_set V F (may_be_static_recv_node_label V e) e \<Longrightarrow>
   (V, C) \<Turnstile>\<^sub>e e \<Longrightarrow>
   ([[] \<mapsto> \<langle>e;Map.empty;[]\<rangle>], {}) \<rightarrow>* (\<E>', H') \<Longrightarrow> 
   every_two_dynamic_paths (is_send_path \<E>' (Ch \<pi> xC)) op =
 "
- apply (simp add: every_two_dynamic_paths.simps every_two_static_paths.simps singular.simps; auto)
+ apply (simp add: every_two_dynamic_paths.simps every_two.simps singular.simps; auto)
  apply (frule_tac \<pi>Sync = \<pi>\<^sub>1 in isnt_send_path_sound; auto)
  apply (drule_tac x = pathSync in spec)
  apply (frule_tac \<pi>Sync = \<pi>\<^sub>2 in isnt_send_path_sound; auto?)
  apply (drule_tac x = pathSynca in spec)
  apply (erule impE, simp)
- apply (simp add: send_static_paths_equal_exclusive_implies_dynamic_paths_equal)
+ apply (simp add: send_abstract_paths_equal_exclusive_implies_dynamic_paths_equal)
 done
-
 
 theorem one_shot_sound: "
   \<lbrakk>
@@ -1972,12 +1141,13 @@ theorem one_shot_sound: "
  apply (simp add: one_shot_sound')
 done
 
+
 (*
 TO DO LATER:
 *)
 
 theorem noncompetitive_send_to_ordered_send: "
-  every_two_static_paths (may_be_static_live_path V F Ln Lx (NLet xC) (may_be_static_send_node_label V e xC)) noncompetitive \<Longrightarrow>
+  every_two (may_be_static_live_path V F Ln Lx (NLet xC) (may_be_static_send_node_label V e xC)) noncompetitive \<Longrightarrow>
   static_chan_liveness V Ln Lx xC e \<Longrightarrow>
   static_flow_set V F (may_be_static_recv_node_label V e) e \<Longrightarrow>
   (V, C) \<Turnstile>\<^sub>e e \<Longrightarrow>
@@ -2004,7 +1174,7 @@ theorem fan_out_sound: "
 done
 
 lemma noncompetitive_recv_to_ordered_recv: "
-   every_two_static_paths (may_be_static_live_path V F Ln Lx (NLet xC) (may_be_static_recv_node_label V e xC)) noncompetitive \<Longrightarrow>
+   every_two (may_be_static_live_path V F Ln Lx (NLet xC) (may_be_static_recv_node_label V e xC)) noncompetitive \<Longrightarrow>
    static_flow_set V F (may_be_static_recv_node_label V e) e \<Longrightarrow>
    (V, C) \<Turnstile>\<^sub>e e \<Longrightarrow>
    ([[] \<mapsto> \<langle>e;Map.empty;[]\<rangle>], {}) \<rightarrow>* (\<E>', H') \<Longrightarrow>
@@ -2044,6 +1214,15 @@ done
 
 
 (*
+
+
+
+lemma paths_cong_preserved_under_reduction: "
+  paths_congruent (\<pi> ;; l) (path @ [n]) \<Longrightarrow>
+  paths_congruent \<pi> path"
+using paths_congruent.cases by fastforce
+
+
 lemma paths_cong_mod_chan_preserved_under_reduction: "
 (suffix \<pi> (\<pi>C ;; (LNext xC)) \<and> suffix path [(NLet xC, ENext)] \<or>
   True) \<Longrightarrow>
@@ -2154,6 +1333,29 @@ proof -
   qed
 qed
 *)
+
+
+(*
+lemma paths_cong_mod_chan_preserved_under_reduction_chan: "
+  paths_congruent ((LNext xC) # \<pi>Suff ;; l) (path @ [n]) \<Longrightarrow>
+  E (\<pi>C @ (LNext xC) # \<pi>Suff) \<noteq> None \<Longrightarrow>
+  paths_congruent_mod_chan (E, H) (Ch \<pi>C xC) (\<pi>C @ (LNext xC) # \<pi>Suff) path"
+using paths_cong_preserved_under_reduction paths_congruent_mod_chan.Chan by blast
+
+lemma  paths_cong_mod_chan_preserved_under_reduction_sync: "
+  paths_congruent (\<pi>Suffix ;; l) (pathSuffix @ [n]) \<Longrightarrow>
+  \<E> (\<pi>R @ (LNext xR) # \<pi>Suffix) \<noteq> None \<Longrightarrow>
+  dynamic_built_on_chan_var \<rho>RY c xR \<Longrightarrow>
+  \<E> \<pi>S = Some (\<langle>LET xS = SYNC xSE in eSY;\<rho>SY;\<kappa>SY\<rangle>) \<Longrightarrow>
+  \<E> \<pi>R = Some (\<langle>LET xR = SYNC xRE in eRY;\<rho>RY;\<kappa>RY\<rangle>) \<Longrightarrow>
+  {(\<pi>S, c, \<pi>R)} \<subseteq> H \<Longrightarrow>
+  paths_congruent_mod_chan (\<E>, H) c \<pi>S pathPre \<Longrightarrow>
+  paths_congruent_mod_chan (\<E>, H) c (\<pi>R @ (LNext xR) # \<pi>Suffix) (pathPre @ (NLet xS, ESend xSE) # (NLet xR, ENext) # pathSuffix)"
+by (meson paths_cong_preserved_under_reduction paths_congruent_mod_chan.Sync)
 *)
+
+
+
+
 
 end
